mostly done w/ Trieber stack, modulo a couple missing axioms

TrieberStack.v
@@ -7,6 +7,21 @@ Require Import RGref.DSL.Concurrency.
     nodes are constant. *)
 Inductive Node : Set :=
   | mkNode : nat -> option (ref{Node|any}[local_imm,local_imm]) -> Node.
+Print ImmediateReachability.
+Global Instance reach_ts_node : ImmediateReachability Node :=
+{ imm_reachable_from_in := fun T P R G r nd =>
+                             match nd with (mkNode n tl) =>
+                                             imm_reachable_from_in r tl
+                             end }.
+Print Containment.
+Global Instance node_contains : Containment Node :=
+{ contains := fun R => True }. (* the recursive refs are heap-agnostic *)
+Print rel_fold.
+Global Instance node_fold : rel_fold Node :=
+{
+  rgfold := fun R G => Node; (* Nodes grant no heap mutation permission to reachable state *)
+  fold := fun R G nd => nd
+}.
 
 (** We'll follow roughly S11.2 of The Art of Multiprocessor Programming:
     a basic Trieber stack, with no backoff or elimination. *)
@@ -26,6 +41,11 @@ Proof.
   eapply ts_pop. rewrite <- H; eauto. constructor. constructor. red. red. reflexivity.
 Qed.
 Hint Resolve precise_deltaTS.
+Lemma hrefl_deltaTS : hreflexive deltaTS.
+Proof.
+  compute. constructor.
+Qed.
+Hint Resolve hrefl_deltaTS.
 
                                                        
 Definition ts := ref{option (ref{Node|any}[local_imm,local_imm])|any}[deltaTS,deltaTS].
@@ -33,4 +53,54 @@ Definition ts := ref{option (ref{Node|any}[local_imm,local_imm])|any}[deltaTS,de
 Program Definition alloc_ts {Γ} (u:unit) : rgref Γ ts Γ :=
   Alloc None.
 
-(* TODO: push, pop implementations *)
+(*Local Obligation Tactic := compute; eauto.*)
+Program Definition push_ts {Γ} : ts -> nat -> rgref Γ unit Γ :=
+  RGFix2 _ _ _ (fun rec s n =>
+    let tl := !s in
+    (* Eventually, lift allocation out of the loop, do substructural
+       allocation, and strongly update tail until insertion *)
+    new_node <- Alloc (mkNode n tl);
+    success <- CAS(s,tl,Some (convert new_node (fun v h (pf:v=mkNode n tl) => I)
+                                               (rel_sub_refl _ local_imm)
+                                               (rel_sub_refl _ local_imm) _ 
+                                               (rel_sub_refl _ local_imm)));
+    if success then rgret tt else rec s n).
+Next Obligation.
+  Admitted. (* Need axiom that ref types are equal if the P, R, and G are all iff *)
+Next Obligation. (* local identity constraint stable wrt local_imm *)
+  compute. intros. subst. rewrite <- H0. reflexivity. Qed.
+Next Obligation.
+  compute; eauto. Qed.
+Next Obligation. (* Guarantee satisfaction! *)
+  unfold push_ts_obligation_8.
+  eapply ts_push. rewrite <- convert_equiv.
+  apply (@heap_lookup2 _ (fun v h => v=mkNode n (!s))).
+Qed.
+
+Program Definition asB T R G B `{rel_fold T} (pf:rgfold R G = B) (b:rgfold R G) : B.
+intros. rewrite pf in b. exact b. Defined.
+Print asB.
+
+Program Definition pop_ts {Γ} : ts -> rgref Γ (option nat) Γ :=
+  RGFix _ _ (fun rec s =>
+    match !s with
+    | None => rgret None
+    | Some hd => match !hd with
+                   | mkNode n tl => 
+                       success <- CAS(s,Some hd,tl);
+                       if success then rgret (Some n) else rec s
+                 end
+    end).
+Next Obligation.
+  Admitted. (* Same axiom need as above *)
+Next Obligation. (* Guarantee Satisfaction *)
+  (* Need to export a couple assumptions locally inside this lemma:*)
+  assert (forall T P R G (r:ref{T|P}[R,G]) B {rf:rel_fold T} rpf (epf:rgfold R G=B), deref rpf epf r = asB R G epf (@fold T _ R G (h[r]))). admit.
+  assert (Hs := H _ _ _ _ s). 
+  assert (Hhd := H _ _ _ _ hd). 
+  erewrite Hhd in Heq_anonymous0. compute in Heq_anonymous0.
+  rewrite Hs in Heq_anonymous. (* <-- Can't finish this compute until I fill in admission above. *)
+  assert (Htemp : Some hd = h[s]). admit.
+  rewrite <- Htemp.
+  eapply ts_pop. symmetry. apply Heq_anonymous0.
+Qed. 
