RGref/DSL/Monad.v
@@ -145,7 +145,14 @@ Notation "VarAlloc! v e" := (varalloc' _ _ _ v e ({{{e}}}) _ _ _ _ _) (at level 
 (** ** Fixpoints *)
 (** Possibly non-terminating fixpoint combinators. *)
 (* TODO: This is only a first cut, and doesn't allow polymorphic recursion. *)
-Axiom RGFix : forall { Γ Γ' }(t t':Set), ((t -> rgref Γ t' Γ') -> (t -> rgref Γ t' Γ')) -> t -> rgref Γ t' Γ'.
-Axiom RGFix2 : forall { Γ Γ' }(t t2 t':Set), ((t -> t2 -> rgref Γ t' Γ') -> (t -> t2 -> rgref Γ t' Γ')) -> t -> rgref Γ t' Γ'.
-Axiom RGFix3 : forall { Γ Γ' }(t t2 t3 t':Set), ((t -> t2 -> t3 -> rgref Γ t' Γ') -> (t -> t2 -> t3 -> rgref Γ t' Γ')) -> t -> rgref Γ t' Γ'.
-Axiom RGFix4 : forall { Γ Γ' }(t t2 t3 t4 t':Set), ((t -> t2 -> t3 -> t4 -> rgref Γ t' Γ') -> (t -> t2 -> t3 -> t4 -> rgref Γ t' Γ')) -> t -> rgref Γ t' Γ'.
+Axiom RGFix : forall { Γ Γ' }(t t':Set), 
+    ((t -> rgref Γ t' Γ') -> (t -> rgref Γ t' Γ')) -> t -> rgref Γ t' Γ'.
+Axiom RGFix2 : forall { Γ Γ' }(t t2 t':Set), 
+    ((t -> t2 -> rgref Γ t' Γ') -> (t -> t2 -> rgref Γ t' Γ')) -> 
+    t -> t2 -> rgref Γ t' Γ'.
+Axiom RGFix3 : forall { Γ Γ' }(t t2 t3 t':Set), 
+    ((t -> t2 -> t3 -> rgref Γ t' Γ') -> (t -> t2 -> t3 -> rgref Γ t' Γ')) -> 
+    t -> t2 -> t3 -> rgref Γ t' Γ'.
+Axiom RGFix4 : forall { Γ Γ' }(t t2 t3 t4 t':Set), 
+    ((t -> t2 -> t3 -> t4 -> rgref Γ t' Γ') -> (t -> t2 -> t3 -> t4 -> rgref Γ t' Γ')) ->
+    t -> t2 -> t3 -> t4 -> rgref Γ t' Γ'.
